Test/File.lean
@@ -44,6 +44,9 @@ inductive FileError where
   | invalidFormat
   | eof
 
+def File.append (f : File) (bs : Array UInt8) : File :=
+  { f with bytes := f.bytes ++ bs, pos := f.pos.castLE (by simp) }
+
 abbrev FileM := EStateM FileError File
 
 namespace FileM
@@ -62,7 +65,7 @@ def read (nbytes : Nat) : FileM (Vector UInt8 nbytes) := do
   return ret
 
 def append (bytes : Array UInt8) : FileM PUnit :=
-  modify fun f => { bytes := f.bytes ++ bytes, pos := f.pos.castLE (by simp[f.pos.isLt]) }
+  modify (·.append bytes)
 
 def tell : FileM Nat := do
   let f ← get
@@ -89,7 +92,7 @@ inductive Schema where
   | byte -- 1 byte
   | word -- 4 bytes, big endian (because)
   | enum (nalts : Nat) (h : nalts ≤ 256) (alts : Fin nalts → Schema)
-  | struct (nflds : Nat) (flds : Fin nflds → Schema)
+--  | struct (nflds : Nat) (flds : Fin nflds → Schema)
   | array (elt : Schema)
 
 def Pi.toTuple (n : Nat) (f : Fin n → Type) : Type := match n with
@@ -100,21 +103,22 @@ abbrev Schema.interp (s : Schema) : Type := match s with
   | byte => UInt8
   | word => UInt32
   | enum nalts _ alts => Σ i : Fin nalts, (alts i).interp
-  | struct nflds flds => Pi.toTuple nflds (fun i => (flds i).interp)
+--  | struct nflds flds => Pi.toTuple nflds (fun i => (flds i).interp)
   | array elt => Array (Schema.interp elt)
 
+mutual
 def Schema.parse (s : Schema) : FileM s.interp := do
   match s with
-  | byte => do
+  | .byte => do
     let b ← FileM.read 1
     return b[0]
-  | word => do
+  | .word => do
     let bs ← FileM.read 4
     let mut ret : UInt32 := 0
     for b in bs do
       ret := ret <<< 8 + b.toUInt32
     return ret
-  | enum nalts _ alts => do
+  | .enum nalts _ alts => do
     let i ← FileM.read 1
     let tag := i[0]
     if h : tag.toNat < nalts
@@ -122,14 +126,8 @@ def Schema.parse (s : Schema) : FileM s.interp := do
       let tag := ⟨tag.toNat, h⟩
       return ⟨tag, ← (alts tag).parse⟩
     else throw FileError.invalidFormat
-  | struct nflds flds => do
-    match h : nflds with
-    | 0 => return ()
-    | nflds + 1 => do
-      let hd ← (flds 0).parse
-      let tl ← (struct nflds (flds ∘ Fin.succ)).parse
-      return (hd, tl)
-  | array elt => do
+--  | .struct nflds flds => Pi.toTuple.parse nflds flds
+  | .array elt => do
     let n ← FileM.read 1
     let n := n[0].toNat
     let mut ret := Array.mkEmpty n
@@ -137,6 +135,16 @@ def Schema.parse (s : Schema) : FileM s.interp := do
       ret := ret.push (← elt.parse)
     return ret
 decreasing_by (repeat sorry)
+
+def Pi.toTuple.parse (n : Nat) (f : Fin n → Schema) : FileM (Pi.toTuple n (Schema.interp ∘ f)) :=
+  match n with
+  | 0 => return ()
+  | n + 1 => do
+    let hd ← (f 0).parse
+    let tl ← Pi.toTuple.parse n (f ∘ Fin.succ)
+    return (hd, tl)
+decreasing_by (repeat sorry)
+end
 
 def Schema.serialize (s : Schema) (v : s.interp) : FileM PUnit := do
   match s, v with
@@ -147,12 +155,12 @@ def Schema.serialize (s : Schema) (v : s.interp) : FileM PUnit := do
   | enum nalts h alts, ⟨tag, v⟩ => do
     FileM.append #[.ofBitVec (tag.castLE h)]
     (alts tag).serialize v
-  | struct nflds flds, t => do
-    match h : nflds with
-    | 0 => return ()
-    | nflds + 1 => do
-      (flds 0).serialize (t.fst)
-      (struct nflds (flds ∘ Fin.succ)).serialize t.snd
+--  | struct nflds flds, t => do
+--    match h : nflds with
+--    | 0 => return ()
+--    | nflds + 1 => do
+--      (flds 0).serialize (t.fst)
+--      (struct nflds (flds ∘ Fin.succ)).serialize t.snd
   | array elt, a => do
     FileM.append #[a.size.toUInt8]
     for (v : elt.interp) in (a : Array elt.interp) do
@@ -162,9 +170,17 @@ decreasing_by (repeat sorry)
 --derive_wp_simp FileM.append
 @[wp_simp]
 theorem FileM.append_apply :
-    wp⟦FileM.append bs⟧.apply Q = fun f => Q.1 ⟨⟩ { f with bytes := f.bytes ++ bs, pos := f.pos.castLE (by simp) } := by
+    wp⟦FileM.append bs⟧.apply Q = fun f => Q.1 ⟨⟩ (f.append bs) := by
   unfold FileM.append
   mstart
+  mwp
+
+-- Same thing as triple:
+theorem FileM.append_spec :
+    ⦃fun f => Q.1 ⟨⟩ { f with bytes := f.bytes ++ bs, pos := f.pos.castLE (by simp) }⦄
+    FileM.append bs
+    ⦃Q⦄ := by
+  mintro _
   mwp
 
 theorem FileM.append_ok : ⦃⌜True⌝⦄ FileM.append bs ⦃⇓ () => ⌜True⌝⦄ := by
@@ -177,9 +193,9 @@ theorem Schema.serialize_ok {s : Schema} (v : s.interp) :
   case case1 => unfold Schema.serialize; mintro - ∀f; mwp
   case case2 => unfold Schema.serialize; mintro - ∀f; mwp
   case case3 ih => unfold Schema.serialize; mintro - ∀f; mwp; mspec ih
-  case case4 ih => unfold Schema.serialize; mintro - ∀f; mwp
-  case case5 ih1 ih2 => unfold Schema.serialize; mintro - ∀f; mwp; mspec ih1; mspec ih2
-  case case6 arr ih =>
+--  case case4 ih => unfold Schema.serialize; mintro - ∀f; mwp
+--  case case5 ih1 ih2 => unfold Schema.serialize; mintro - ∀f; mwp; mspec ih1; mspec ih2
+  case case4 arr ih =>
     unfold Schema.serialize
     mintro - ∀f
     mwp
@@ -188,24 +204,221 @@ theorem Schema.serialize_ok {s : Schema} (v : s.interp) :
     mspec (Specs.foldlM_list (m := FileM) (⇓ _ => ⌜True⌝) ?step)
     case step => intros; apply ih
 
-def Schema.fileSize {s : Schema} (v : s.interp) : Nat :=
-  match EStateM.run (s.serialize v) File.mkEmpty with
-  | .ok _ f => f.bytes.size
-  | .error _ _ => panic! "failed to serialize"
+theorem serialize_ne_error {s : Schema} (v : s.interp) :
+    s.serialize v File.mkEmpty ≠ .error e f := by
+  have := Schema.serialize_ok v File.mkEmpty True.intro
+  simp[wp, FailConds.false, FailConds.const] at this
+  simp[this]
+  intro h
+  simp[h] at this
 
-theorem Triple.conj [WP m ps] (x : m α) (h₁ : ⦃P₁⦄ x ⦃Q₁⦄) (h₂ : ⦃P₂⦄ x ⦃Q₂⦄) : ⦃P₁ ∧ P₂⦄ x ⦃Q₁ ∧ₚ Q₂⦄ := by
-  mintro ⟨hp₁, hp₂⟩
-  mreplace hp₁ : wp⟦x⟧.apply Q₁ := by mspecialize_pure h₁ hp₁ as h; mexact h
-  mreplace hp₂ : wp⟦x⟧.apply Q₂ := by mspecialize_pure h₂ hp₂ as h; mexact h
-  mhave hp : spred(wp⟦x⟧.apply Q₁ ∧ wp⟦x⟧.apply Q₂) := by mrefine ⟨hp₁,hp₂⟩
-  mspecialize_pure ((wp⟦x⟧.conjunctive _ _).mpr) hp as h
-  mexact h
+theorem serialize_ok_simple {s : Schema} (v : s.interp) :
+    ∃ f, s.serialize v File.mkEmpty = .ok () f := by
+  cases h : s.serialize v File.mkEmpty <;> simp_all [serialize_ne_error v]
 
-def Schema.wellFormedSubFile (s : Schema) (f : File) : Prop :=
-  ∃ v : s.interp, match EStateM.run (s.serialize v) File.mkEmpty with
-  | .ok () f0 => f.bytes[f.pos.val : f.pos.val + f0.bytes.size] = f0.bytes
-  | .error _ _ => False
-def Schema.wellFormedSubFile2 (s : Schema) (f : File) : Prop :=
-  ∃ v : s.interp, (s.serialize v) File.mkEmpty with
-  | .ok () f0 => f.bytes[f.pos.val : f.pos.val + f0.bytes.size] = f0.bytes
-  | .error _ _ => False
+def byteSize {s : Schema} (v : s.interp) : Nat :=
+  match s, v with
+  | .byte, _ => 1
+  | .word, _ => 4
+  | .enum _ _ _, ⟨_, v⟩ => 1 + byteSize v
+--  | .struct 0 flds, t => 0
+--  | .struct (n+1) flds, (e, t) => byteSize e + @byteSize (Schema.struct n (flds ∘ Fin.succ)) t
+  | .array _, a => a.foldl (init := 0) (fun acc v => acc + byteSize v)
+
+theorem EStateM.wp_to_tuple {ε σ α} {x : EStateM ε σ α} {Q : PostCond α (.except ε (.arg σ .pure))} {s : σ}
+  (h : wp⟦x⟧.apply Q s) : ⦃(· = s)⦄ x ⦃Q⦄ := by intro _ hs; subst hs; exact h
+
+theorem serialize_byteSize {s : Schema} (v : s.interp) (f : File) :
+  match s.serialize v f with
+  | .ok () f' => f'.bytes.size = byteSize v + f.bytes.size
+  | .error _ _ => False := by
+  generalize h : s.serialize v f = x
+  apply EStateM.by_wp h _
+  subst h
+  simp
+  induction s, v using Schema.serialize.induct generalizing f
+  case case1 => unfold Schema.serialize; mstart; mwp; simp +arith [File.mkEmpty, byteSize]
+  case case2 => unfold Schema.serialize; mstart; mwp; simp +arith [File.mkEmpty, byteSize]
+  case case3 tag v ih =>
+    unfold Schema.serialize
+    mstart
+    mwp
+    mspec (EStateM.wp_to_tuple (ih { bytes := f.bytes.push (OfNat.ofNat ↑tag), pos := Fin.castLE _ f.pos }))
+    case post.success => simp +arith [File.mkEmpty, byteSize, *]
+    simp +arith [File.mkEmpty, byteSize, *]
+  case case4 arr ih =>
+    unfold Schema.serialize
+    mstart
+    mwp
+    cases arr
+    conv in forIn _ _ _ => simp
+    mspec (Specs.foldlM_list (⇓ _ => ⌜True⌝) ?step)
+    case step => intros; apply ih
+
+  unfold Schema.serialize
+  mstart
+  mwp
+  simp[File.mkEmpty]
+
+theorem test {s : Schema} (v : s.interp) (f : File)
+  (case1 : ∀ (v : Schema.byte.interp) (f : File), Q.1 () (f.append #[v]))
+  (case2 : ∀ (v : Schema.word.interp) (f : File), Q.1 () (f.append <| #[v >>> 24, v >>> 16, v >>> 8, v].map (·.toUInt8)))
+  (case3 : ∀ (elt : Schema) (v : (Schema.array elt).interp) (f : File),
+           ∃ (I : PostCond (PUnit × List.Zipper v.toList) (.except FileError (.arg File .pure))),
+             (I.1 ((), ⟨[], v.toList, by simp⟩) (f.append #[v.size.toUInt8]))
+             ∧ (I.1 ((), ⟨v.toList.reverse, [], by simp⟩) ⊢ₛ Q.1 ())
+             ∧ (I.2 ⊢ₑ Q.2))
+  :
+  wp⟦s.serialize v⟧.apply Q f := by
+  apply Schema.serialize.fun_cases _ ?case1 ?case2 ?case3 ?case4 s v
+  case case1 => unfold Schema.serialize; mstart; mwp; mpure_intro; intro v; apply case1
+  case case2 => unfold Schema.serialize; mstart; mwp; mpure_intro; intro v; apply case2
+  case case3 =>
+    intro nalt h alts tag v
+    unfold Schema.serialize
+    mstart
+    mwp
+    mpure_intro
+    exact test v (f.append #[OfNat.ofNat tag]) case1 case2 case3
+  case case4 =>
+    intro elt arr
+    unfold Schema.serialize
+    mstart
+    mwp
+    have ⟨I, hpre, hpost, hexcept⟩ := case3 elt arr f
+    -- conv in forIn _ _ _ => simp
+    -- mspec (Specs.foldlM_list (⇓ (_, xs) => ⌜True⌝) ?step)
+    mspec_no_bind Specs.forIn_array
+    case inv => exact I
+    case pre => simp[hpre]
+    case post.success => simp[hpost]
+    case post.except.handle => simp[hexcept.1]
+    case step =>
+      intro _ _ v _ _
+      mintro h ∀f
+      mwp
+      mcases h with ⌜hinv⌝
+      mpure_intro
+      refine test v f ?case1 ?case2 ?case3
+      case case1 => simp
+
+  ·
+  match s, v using Schema.serialize. generalizing Q f
+  induction s, v using Schema.serialize.induct generalizing Q f
+  case case1 => unfold Schema.serialize; mstart; mwp; mpure_intro; apply case1
+  case case2 => unfold Schema.serialize; mstart; mwp; mpure_intro; apply case2
+  case case3 tag v ih =>
+    unfold Schema.serialize
+    mstart
+    mwp
+    mspec (EStateM.wp_to_tuple (ih (f.append #[OfNat.ofNat tag])))
+  case case4 elt arr ih =>
+    unfold Schema.serialize
+    mstart
+    mwp
+    have ⟨I, hpre, hpost, hexcept⟩ := case3 elt arr f
+    -- conv in forIn _ _ _ => simp
+    -- mspec (Specs.foldlM_list (⇓ (_, xs) => ⌜True⌝) ?step)
+    mspec_no_bind Specs.forIn_array
+    case inv => exact I
+    case pre => simp[hpre]
+    case post.success => simp[hpost]
+    case post.except.handle => simp[hexcept.1]
+    case step =>
+      intros
+      mintro h
+      mwp
+
+  unfold Schema.serialize
+  mstart
+  mwp
+  simp[File.mkEmpty]
+
+theorem byteSize_byte : byteSize (b : Schema.byte.interp) = 1 := by
+  simp [byteSize]
+  generalize h : Schema.serialize Schema.byte b File.mkEmpty = x
+  apply EStateM.by_wp h
+  unfold Schema.serialize
+  mstart
+  mwp
+  simp[File.mkEmpty]
+
+def serialized {s : Schema} (v : s.interp) (f : File) : Prop :=
+  match h : s.serialize v File.mkEmpty with
+  | .ok () f0 => f0.bytes.size = byteSize v ∧ f.bytes.extract f.pos.val (f.pos.val + byteSize v) = f0.bytes
+  | .error _ _ => False.elim (serialize_ne_error v h)
+
+def canRead (n : Nat) (f : File) : Prop :=
+  f.pos + n ≤ f.bytes.size
+
+def hasRead {n : Nat} (v : Vector UInt8 n) (f : File) : Prop :=
+  f.bytes.extract (f.pos - n) f.pos = v.toArray
+
+theorem Array.extract_size_eq {a : Array α} {start : Nat} :
+    start ≤ a.size → (a.extract start (start + n)).size = n → start + n ≤ a.size := by
+  simp +contextual +arith
+  intro h
+  omega
+
+theorem serialized_canRead {s : Schema} (v : s.interp) :
+    SPred.entails (σs:=[File]) (serialized v) (canRead (byteSize v)) := by
+  intro f
+  simp [serialized, canRead]
+  intro h
+  split at h
+  case h_2 heq => exfalso; exact serialize_ne_error v heq
+  rcases h with ⟨h₁, h₂⟩
+  rw[← h₂] at h₁
+  have := Array.extract_size_eq (Nat.le_of_lt_add_one f.pos.isLt) h₁
+  simp_all
+
+@[grind →]
+theorem range_elim : List.range' s n = xs ++ i :: ys → i = s + xs.length := by
+  intro h
+  induction xs generalizing s n
+  case nil => cases n <;> simp_all[List.range']
+  case cons head tail ih =>
+    cases n <;> simp[List.range'] at h
+    have := ih h.2
+    simp[ih h.2]
+    omega
+
+@[spec]
+theorem read_spec :
+  ⦃canRead n⦄ FileM.read n ⦃⇓ v => hasRead v⦄ := by
+  mintro h ∀f
+  unfold FileM.read
+  mwp
+  mspec (Specs.forIn'_list ?inv ?step)
+  case inv => exact ⇓ (⟨pos, buf⟩, xs) =>
+    ⌜pos = f.pos + xs.pref.length ∧ pos + xs.suff.length ≤ f.bytes.size
+    ∧ f.bytes.extract f.pos pos = buf.toArray.take xs.pref.length⌝
+  case pre => simp +contextual [canRead]; omega
+  case step =>
+    intro ⟨pos, buf⟩ pref i hi suff hsuff
+    have := range_elim hsuff
+    simp at this
+    subst_vars
+    mintro ⌜hinv⌝
+    simp at hinv
+    mwp
+    split
+    · mpure_intro
+      simp +arith [hinv]
+      sorry -- pure proof about offset arithmetic
+    · simp_all
+      omega
+  case post.except.handle => simp
+  mintro ∀f
+  simp_all [hasRead]
+
+theorem blah {s : Schema} (v : s.interp) :
+    ⦃serialized v⦄
+    s.parse
+    ⦃⇓ v' => ⌜v = v'⌝⦄ := by
+  mintro hser
+  induction s using Schema.parse.induct
+  case case1 =>
+    unfold Schema.parse
+    mspec read_spec
+    case pre => simp [serialized_canRead]
