MPL/Triple.lean
@@ -25,6 +25,8 @@ variable {m : Type → Type u} {ps : PostShape} [WP m ps]
 def Triple (x : m α) (P : Assertion ps) (Q : PostCond α ps) : Prop :=
   P ⊢ₛ wp⟦x⟧.apply Q
 
+namespace Triple
+
 notation:lead "⦃" P "⦄ " x:lead " ⦃" Q "⦄" => Triple x spred(P) spred(Q)
 app_unexpand_rule Triple
   | `($_ $x $P $Q) => match Q with
@@ -36,18 +38,25 @@ app_unexpand_rule Triple
 instance [WP m ps] (x : m α) : ProofMode.PropAsEntails (Triple x P Q) spred(P → wp⟦x⟧.apply Q) where
   prop_as_entails := (SPred.entails_true_intro P (wp⟦x⟧.apply Q)).symm
 
-theorem Triple.pure [Monad m] [MonadMorphism m (PredTrans ps) wp] {α} {Q : PostCond α ps} (a : α) (himp : P.entails (Q.1 a)) :
+theorem pure [Monad m] [MonadMorphism m (PredTrans ps) wp] {α} {Q : PostCond α ps} (a : α) (himp : P.entails (Q.1 a)) :
   Triple (pure (f:=m) a) P Q := himp.trans (by simp only [pure_pure, PredTrans.pure_apply, SPred.entails.refl])
 
-theorem Triple.bind [Monad m] [MonadMorphism m (PredTrans ps) wp] {α β} {P : Assertion ps} {Q : α → Assertion ps} {R : PostCond β ps} (x : m α) (f : α → m β)
-  (hx : Triple x P (Q, R.2))
-  (hf : ∀ b, Triple (f b) (Q b) R) :
-  Triple (x >>= f) P R := by
-    apply SPred.entails.trans hx
-    simp only [bind_bind]
-    apply wp⟦x⟧.mono _ _
-    simp only [PostCond.entails, Assertion, FailConds.entails.refl, and_true]
-    exact hf
+theorem bind [Monad m] [MonadMorphism m (PredTrans ps) wp] {α β} {P : Assertion ps} {Q : α → Assertion ps} {R : PostCond β ps} (x : m α) (f : α → m β)
+    (hx : Triple x P (Q, R.2))
+    (hf : ∀ b, Triple (f b) (Q b) R) :
+    Triple (x >>= f) P R := by
+  apply SPred.entails.trans hx
+  simp only [bind_bind]
+  apply wp⟦x⟧.mono _ _
+  simp only [PostCond.entails, Assertion, FailConds.entails.refl, and_true]
+  exact hf
 
-theorem Triple.and (x : m α) (h₁ : ⦃P₁⦄ x ⦃Q₁⦄) (h₂ : ⦃P₂⦄ x ⦃Q₂⦄) : ⦃P₁ ∧ P₂⦄ x ⦃Q₁ ∧ₚ Q₂⦄ :=
+theorem and (x : m α) (h₁ : ⦃P₁⦄ x ⦃Q₁⦄) (h₂ : ⦃P₂⦄ x ⦃Q₂⦄) : ⦃P₁ ∧ P₂⦄ x ⦃Q₁ ∧ₚ Q₂⦄ :=
   (SPred.and_mono h₁ h₂).trans (wp⟦x⟧.conjunctive Q₁ Q₂).mpr
+
+end Triple
+
+theorem EStateM.by_triple {α} {x : EStateM.Result ε σ α} {prog : EStateM ε σ α} (h : EStateM.run prog s = x) (P : EStateM.Result ε σ α → Prop) :
+    ⦃(· = s)⦄ prog ⦃⇓ a s' => P (EStateM.Result.ok a s')⦄ → P x := by
+  intro hspec
+  exact EStateM.by_wp h P (hspec s rfl)
